Fixed syntax (builtin), first self-built tactic for multiplication

lib/basics.v
@@ -17,29 +17,13 @@ Fixpoint subst (x : string) (s : exp) (t : exp) : exp :=
       <{(/x:=s/ t1) (/x:=s/ t2)}>
   | <{val n = t1 ; t2}> =>
       if (String.eqb x n) then t else <{val n = (/x:=s/ t1) (*Dentro n non si può sostituire ?*) ; (/x:=s/ t2)}>
-  | exp_nvalue w =>
-    <{w}>
-  | <{true}> =>
-      <{true}>
-  | <{false}> =>
-      <{false}>
-  | l_const n =>
-    <{n}>
-  | l_succ t1 =>
-    <{succ (/x:=s/ t1)}>
-  | l_pred t1 =>
-    <{pred (/x:=s/ t1)}>
-  | l_mult w0 w1 =>
-    <{w0 * w1}>
-  | l_uid => 
-      l_uid
-  | l_self w0 =>
-      <{self w0 }> 
-  | l_sensor s =>
-      l_sensor s
+  | l_builtin b => l_builtin b
+  | l_sensor s => l_sensor s
+  | l_true => l_true
+  | l_false => l_false
+  | l_const n => l_const n
   | l_fail => l_fail
-  | l_nfold w0 w1 w2 => l_nfold <{/x:=s/ w0}> <{/x:=s/w1}> <{/x:=s/w2}>
-  | l_exchange w0 w1 => l_exchange <{/x:=s/w0}> <{/x:=s/w1}>
+  | exp_nvalue w => <{w}>
 end
 where "'/' x ':=' s '/' t" := (subst x s t) (in custom acnotation).
 
@@ -49,43 +33,26 @@ Fixpoint bounded (e:exp) (l_bounded:list string) {struct e}: Prop :=
 let l_b := 
   (fix l_b (l : literal) : Prop := 
         match l with
-        | l_uid =>
-          True
-        | l_self w0 => 
-          bounded w0 nil
-        | l_sensor s => 
-            True
+        | l_builtin b => True
+        | <{fun n [y:T] {t1}}> => 
+              bounded t1 (cons y l_bounded)
+        | l_sensor s => True
         | l_fail => False
-        | <{true}> =>
-          False
-        | <{false}> =>
-          True
-        | l_const n =>
-          True
-        | l_succ t1 =>
-          (bounded t1 l_bounded)
-        | l_pred t1 =>
-          (bounded t1 l_bounded)
-        | l_mult w1 w2 =>
-            bounded w1 nil /\ bounded w2 nil
-        | <{fun n [y:T] {t1}}> =>
-            bounded t1 (cons y l_bounded)
-        | l_nfold w0 w1 w2 => 
-            bounded w0 nil /\ bounded w1 nil /\ bounded w2 nil 
-        | l_exchange w0 w1=> 
-            bounded w0 nil /\ bounded w1 nil 
+        | l_true => True
+        | l_false => True
+        | l_const n => True
         end
     )
 in
 match e with 
   | exp_var y =>
     In y l_bounded
-  | <{fun n [y:T] {t1}}> =>
-    bounded t1 (cons y l_bounded)
   | <{t1 t2}> =>
-    (bounded t1 l_bounded) /\ (bounded t1 l_bounded)
+    (bounded t1 l_bounded) /\ (bounded t2 l_bounded)
   | <{val n = t1 ; t2}> =>
     (bounded t1 l_bounded) /\ (bounded t2 (cons n l_bounded))
+  | <{fun n [y:T] {t1}}> =>
+    bounded t1 (cons y l_bounded)
   | exp_nvalue w =>
     (fix w_rec (w : nvalue ) : Prop := 
     match w with
@@ -95,22 +62,15 @@ match e with
   | exp_literal l => l_b l
 end.
 
-
-Inductive value : literal -> Prop :=
-  | v_abs : forall n x T2 t1, bounded <{fun n [x:T2] {t1}}> nil ->
-      value <{fun n [x:T2] {t1}}>
-  | v_true :
-      value <{true}>
-  | v_false :
-      value <{false}>
-  | v_nat: forall (n:nat), value <{n}>.
-Hint Constructors value : core.
-
+(*
 Inductive w_values : nvalue -> Prop :=
-| w_default : forall v, value v -> w_values (default v)
-| w_device : forall n v wl, value v -> w_values wl -> w_values (device n v wl).
+| w_default : forall l, bounded (exp_literal l) nil-> w_values (default l)
+| w_device : forall n l wl, bounded (exp_literal l) nil -> w_values wl -> w_values (device n l wl).
+*)
 
-Definition w_value (w:nvalue):= ordered w /\ w_values w.
+Definition value (l:literal) : Prop := bounded (exp_literal l) nil.
+
+Definition w_value (w:nvalue):= ordered w /\ bounded (exp_nvalue w) nil.
 
 Inductive is_fun: exp -> Prop :=
   | func : forall n x T2 t1, 
