acomputing/syntax.v
@@ -17,6 +17,7 @@ Inductive ty : Type :=
   | Ty_Builtin : Type -> ty
   | Ty_Arrow : ty -> ty -> ty.
 
+
 (** SYNTAX of an EXPRESSION, including LITERALS and NVALUES*)
 (** An expression can be a 
 variable (rappresented by string), .... *)
@@ -24,25 +25,27 @@ Inductive exp: Type :=
   | exp_var : string -> exp
   | exp_app : exp -> exp -> exp
   | exp_val : string -> exp -> exp -> exp
-  | exp_nvalue : nvalue -> exp
   | exp_literal : literal -> exp
+  | exp_nvalue : nvalue -> exp
 with literal :=
-  | l_self: exp -> literal
-  | l_uid: literal
+  | l_builtin : builtin -> literal
+  | l_abs : string -> string -> ty -> exp -> literal 
   | l_sensor: string -> literal
   | l_fail : literal
   | l_true : literal
   | l_false : literal
   | l_const : nat -> literal
-  | l_succ : exp -> literal
-  | l_pred : exp -> literal 
-  | l_abs : string -> string -> ty -> exp -> literal 
-  | l_mult : exp -> exp -> literal
-  | l_nfold : exp -> exp -> exp -> literal
-  | l_exchange : exp -> exp -> literal
 with nvalue :=
   | default: literal -> nvalue
-  | device (n:ident) : literal -> nvalue -> nvalue.
+  | device (n:ident) : literal -> nvalue -> nvalue
+with builtin :=
+  | b_exchange : builtin
+  | b_nfold : builtin
+  | b_self: builtin
+  | b_uid: builtin
+  | b_succ : builtin
+  | b_pred : builtin 
+  | b_mult : builtin.
 
 Declare Custom Entry acnotation.
 
@@ -70,33 +73,22 @@ Notation "'val' name = x ; y" := (exp_val name x y) (in custom acnotation at lev
                                                     left associativity).
 
 Notation "S -> T" := (Ty_Arrow S T) (in custom acnotation at level 50, right associativity).
-
+Notation "'Nat'" := (Ty_Builtin nat) (in custom acnotation at level 0).
 Notation "'Bool'" := (Ty_Builtin bool) (in custom acnotation at level 0).
+
 Notation "'true'" := true (at level 1).
 Notation "'true'" := l_true (in custom acnotation at level 0).
 Notation "'false'" := false (at level 1).
 Notation "'false'" := l_false (in custom acnotation at level 0).
 
-(*natural numbers*)
-Notation "'Nat'" := (Ty_Builtin nat) (in custom acnotation at level 0).
-Notation "'succ' x" := (l_succ x) (in custom acnotation at level 0,
-                                     x custom acnotation at level 0).
-Notation "'pred' x" := (l_pred x) (in custom acnotation at level 0,
-                                     x custom acnotation at level 0).
-Notation "x * y" := (l_mult x y) (in custom acnotation at level 1,
-                                      left associativity).
+Notation "'exchange'" := (b_exchange) (in custom acnotation at level 0).
+Notation "'nfold'" := (b_nfold) (in custom acnotation at level 0).
+Notation "'self'" := (b_self) (in custom acnotation at level 0).
+Notation "'uid'" := (b_uid) (in custom acnotation at level 0).
+Notation "'succ'" := (b_succ) (in custom acnotation at level 0).
+Notation "'pred'" := (b_pred) (in custom acnotation at level 0).
+Notation "'mult'" := (b_mult) (in custom acnotation at level 0).
 
-Notation "'nfold' e0 e1 e2" := (l_nfold e0 e1 e2) (in custom acnotation at level 0,
-                                     e0 custom acnotation at level 0,
-                                     e1 custom acnotation at level 0,
-                                     e2 custom acnotation at level 0).
-
-Notation "'exchange' e0 e1" := (l_exchange e0 e1) (in custom acnotation at level 0,
-                                     e0 custom acnotation at level 0,
-                                     e1 custom acnotation at level 0).
-
-
-(*nvalues*)
 Notation "[ > l ]" := (default l) (in custom acnotation at level 30).
 Notation "[ x >> y ] m" := ( device x y m)(in custom acnotation at level 30,
                                             x at level 99, 
@@ -107,12 +99,9 @@ Notation "'FAIL'" := (l_fail) (in custom acnotation at level 0).
 
 Notation "'sensor' x" := (l_sensor x) (in custom acnotation at level 0, x custom acnotation at level 0).
 
-Notation "'self' x" := (l_self x) (in custom acnotation at level 0, x custom acnotation at level 0).
 
-Notation "'uid'" := (l_uid) (in custom acnotation at level 0).
-
-(** EXPRESS CONCEPT*)
 Coercion exp_var : string >-> exp.
+Coercion l_builtin : builtin >-> literal.
 Coercion exp_literal: literal >-> exp.
 Coercion l_const: nat >-> literal.
 Coercion exp_nvalue: nvalue >-> exp.
