acomputing/tactics.v
@@ -1,0 +1,25 @@
+From AC Require Import syntax.
+From AC Require Import basics.
+From AC Require Import sensor_state.
+From AC Require Import value_tree.
+From AC Require Import nvalues.
+From AC Require Import big_step_semantics.
+Require Import Bool.
+Require Import String.
+Require Import List.
+Require Import PeanoNat.
+
+Ltac ordered_tac := first [apply ordered0 | apply ordered1 | apply ordered2;auto;ordered_tac].
+Ltac w_tac := split; [>ordered_tac | simpl;auto].
+
+Ltac mult_tac  := 
+apply A_MULT;
+match goal with
+| [|- w_value ?X] => w_tac
+| _ => apply E_NVAL; w_tac
+end.
+
+Lemma multiplication: <[ 10 | base | vt_end |   <{mult ([1>>5][2>>5][>5]) ([1>>5][>6]) }> ]> ==> <[ <{ [1>>25][2>>30][>30]}> | empty nil ]>.
+Proof.
+mult_tac.
+Qed.
