test/basics_test.v
@@ -14,24 +14,24 @@ Definition fun1: string := "fun1".
 Definition prod5: string := "prod5". 
 
 Check <{x}>.
-Check <{fun prod5 [x:Nat] {x * [>5]} 5}>.
-Check <{x (fun prod5 [x:Nat] {x * 5})}>.
-Check <{val n = 25 ; n * 2}>.
+Check <{fun prod5 [x:Nat] {mult x ([>5])} 5}>.
+Check <{x (fun prod5 [x:Nat] {mult x 5})}>.
+Check <{val n = 25 ; mult n 2}>.
 Check <{[4 >> 2][5 >> 5][6 >> 4][ > 5]}>.
 Check <{uid}>.
-Check <{self [>6]}>.
+Check <{self ([>6])}>.
 Check <{sensor x}>.
 Check <{FAIL}>.
-Check <{nfold [> fun fun1 [x:Nat] {fun fun0  [y:Nat] {x}} ] [0 >> 5][1 >> 3][ > 4 ] [> 5]}>.
+Check <{nfold ([> fun fun1 [x:Nat] {fun fun0  [y:Nat] {x}}]) ([0 >> 5][1 >> 3][ > 4 ]) ([> 5])}>.
 
 
-Compute (<{/x:=5/ (x * y)}>).
+Compute (<{/x:=5/ (mult x y)}>).
 
-Compute (<{ /y:=10/ fun prod5 [x:Nat] {x * y * [>5]} 5}>).
+Compute (<{ /y:=10/ fun prod5 [x:Nat] {mult x (mult y ([>5])) } }>).
 
-Compute <{/x:=4/ (x (fun prod5 [x:Nat] {x * 5}))}>.
+Compute <{/x:=4/ (x (fun prod5 [x:Nat] {mult x 5}))}>.
 
-Compute <{/prod5:=4/ (x (fun prod5 [x:Nat] {x * 5}))}>.
+Compute <{/prod5:=4/ (x (fun prod5 [x:Nat] {mult x 5}))}>.
 
 Compute (bounded <{x}> nil).
 
@@ -50,19 +50,19 @@ Proof.
 simpl. split. left. auto. auto. 
 Qed.
 
-Lemma test4 : bounded <{[0 >> (fun fun0 [x:Nat] {x*y})][>5]}> nil.
+Lemma test4 : bounded <{[0 >> (fun fun0 [x:Nat] {mult x y})][>5]}> nil.
 Proof.
 simpl. split. split. auto. 
 Abort.
 
-Lemma test4 : bounded <{nfold [0 >> (fun fun0 [x:Nat] {x*y})][>5] [>6] [>([>1] * [>(fun fun0 [x:Nat] {y})])] }> nil.
+Lemma test4 : bounded <{nfold ([0 >> (fun fun0 [x:Nat] {mult x y})][>5]) ([0>>5][>6]) ([>6]) }> nil.
 Proof.
 simpl. split. split. split. auto. 
 Abort.
 
 Lemma w_test0 : w_value <{[>3]}>.
 Proof.
-split. apply ordered0. apply w_default. apply v_nat.
+split. apply ordered0. simpl. auto.
 Qed.
 
 Lemma w_test1 : w_value <{[3 >> 2][2 >> 4][>3]}>.
@@ -74,7 +74,6 @@ Lemma w_test2 :  w_value <{[1 >> (fun fun0 [x:Nat] {y})][2 >> 4][>3]}>.
 Proof.
 split. 
 - apply ordered2. auto. apply ordered1. 
-- apply w_device.
-+ apply v_abs. simpl. left. 
+- simpl.
 Abort.
 
